ugh

DenotSem/Values.thy
@@ -5,6 +5,8 @@ begin
 datatype val = VNat nat | VFun "entry list" and
   entry = Entry val val (infix "\<mapsto>" 70)
 
+type_synonym func = "entry list"  
+  
 inductive consistent :: "val \<Rightarrow> val \<Rightarrow> bool" (infix "~" 52) and
     inconsistent :: "val \<Rightarrow> val \<Rightarrow> bool" (infix "!~" 52) where
   vnat_consis[intro!]: "(VNat n) ~ (VNat n)" |
@@ -15,14 +17,31 @@ inductive consistent :: "val \<Rightarrow> val \<Rightarrow> bool" (infix "~" 52
                          \<Longrightarrow> (VFun t1) !~ (VFun t2)" |
   vnat_vfun_inconsis[intro!]: "VNat n !~ VFun t" |
   vfun_vnat_inconsis[intro!]: "VFun t !~ VNat n"
+  
+inductive_cases 
+  vnat_consis_inv[elim!]: "VNat n ~ VNat n'" and
+  vfun_consis_inv[elim!]: "VFun t ~ VFun t'" and
+  vnat_inconsis_inv[elim!]: "VNat n !~ VNat n'" and
+  vfun_inconsis_inv[elim!]: "VFun t !~ VFun t'" and
+  vnat_vfun_consis_inv[elim!]: "VNat n ~ VFun t" and
+  vfun_vnat_consis_inv[elim!]: "VFun t ~ VNat n"
+  
+inductive consis_env :: "val list \<Rightarrow> val list \<Rightarrow> bool" where
+  consis_env_nil[intro!]: "consis_env [] []" |
+  consis_env_cons[intro!]: "\<lbrakk> v ~ v'; consis_env \<rho> \<rho>' \<rbrakk> \<Longrightarrow> consis_env (v#\<rho>) (v'#\<rho>')" 
 
-definition is_fun :: "entry list \<Rightarrow> bool" where
+definition is_fun :: "func \<Rightarrow> bool" where
   "is_fun t \<equiv> (\<forall> v1 v2 v1' v2'. v1\<mapsto>v1' \<in> set t \<and> v2\<mapsto>v2' \<in> set t \<and> v1 ~ v2 \<longrightarrow> v1' ~ v2')"
     
 inductive is_val :: "val \<Rightarrow> bool" where
   vnat_is_val[intro!]: "is_val (VNat n)" |
   vfun_is_val[intro!]: "\<lbrakk> is_fun t; \<forall> v v'. v\<mapsto>v' \<in> set t \<longrightarrow> is_val v \<and> is_val v' \<rbrakk>
                         \<Longrightarrow> is_val (VFun t)"
+inductive_cases
+  vfun_is_val_inv[elim!]: "is_val (VFun t)"
+
+definition val_env :: "val list \<Rightarrow> bool" where
+  "val_env \<rho> \<equiv> \<forall>k. k < length \<rho> \<longrightarrow> is_val (\<rho>!k)"
   
 fun val_join :: "val \<Rightarrow> val \<Rightarrow> val" (infix "\<squnion>" 56) where
   "VNat n1 \<squnion> VNat n2 = (if n1 = n2 then VNat n1 else undefined)" |
@@ -36,8 +55,8 @@ fun env_join :: "val list \<Rightarrow> val list \<Rightarrow> val list" (infix 
 
 inductive val_le :: "val \<Rightarrow> val \<Rightarrow> bool" (infix "\<sqsubseteq>" 52) and
     entry_le :: "entry \<Rightarrow> entry \<Rightarrow> bool" (infix "\<sqsubseteq>" 52) and
-    fun_le :: "entry list \<Rightarrow> entry list \<Rightarrow> bool" (infix "\<sqsubseteq>" 52) and
-    fun_in :: "entry \<Rightarrow> entry list \<Rightarrow> bool" ("_ in _" [56,56] 55)
+    fun_le :: "func \<Rightarrow> func \<Rightarrow> bool" (infix "\<sqsubseteq>" 52) and
+    fun_in :: "entry \<Rightarrow> func \<Rightarrow> bool" ("_ in _" [56,56] 55)
     where
   vnat_le[intro!]: "(VNat n) \<sqsubseteq> (VNat n)" |
   vfun_le[intro!]: "t1 \<sqsubseteq> t2 \<Longrightarrow> (VFun t1) \<sqsubseteq> (VFun t2)" |
@@ -51,9 +70,8 @@ inductive val_le :: "val \<Rightarrow> val \<Rightarrow> bool" (infix "\<sqsubse
                    \<Longrightarrow> (v,v') in t"
 *)
   
-inductive env_le :: "val list \<Rightarrow> val list \<Rightarrow> bool" (infix "\<sqsubseteq>" 52) where
-  empty_env_le[intro!]: "([]::val list) \<sqsubseteq> []" |
-  cons_env_le[intro!]: "\<lbrakk> (v::val) \<sqsubseteq> v'; \<rho> \<sqsubseteq> \<rho>' \<rbrakk> \<Longrightarrow> (v#\<rho>) \<sqsubseteq> (v'#\<rho>')"
+definition env_le :: "val list \<Rightarrow> val list \<Rightarrow> bool" (infix "\<sqsubseteq>" 52) where 
+  "(\<rho>::val list) \<sqsubseteq> \<rho>' \<equiv> length \<rho> = length \<rho>' \<and> (\<forall> k. k < length \<rho>  \<longrightarrow> \<rho>!k \<sqsubseteq> \<rho>'!k)" 
 
 inductive_cases 
   le_fun_fun_inv[elim!]: "VFun t1 \<sqsubseteq> VFun t2" and
@@ -62,8 +80,7 @@ inductive_cases
   le_nat_any_inv[elim!]: "VNat n \<sqsubseteq> v" and
   le_fun_any_inv[elim!]: "VFun t \<sqsubseteq> v" and
   le_any_fun_inv[elim!]: "v \<sqsubseteq> VFun t" and
-  le_cons_fun_inv[elim!]: "((p::entry)#t1) \<sqsubseteq> t2" and
-  le_cons_env_inv[elim!]: "((v::val)#\<rho>) \<sqsubseteq> (v'#\<rho>')"
+  le_cons_fun_inv[elim!]: "((p::entry)#t1) \<sqsubseteq> t2"
   
 section "Joins and Meets"
   
@@ -72,5 +89,14 @@ abbreviation val_lub :: "val \<Rightarrow> val \<Rightarrow> val \<Rightarrow> b
 
 abbreviation val_glb :: "val \<Rightarrow> val \<Rightarrow> val \<Rightarrow> bool" where
   "val_glb v v1 v2 \<equiv> v \<sqsubseteq> v1 \<and> v \<sqsubseteq> v2 \<and> (\<forall> v'. v' \<sqsubseteq> v1 \<and> v' \<sqsubseteq> v2 \<longrightarrow> v' \<sqsubseteq> v)"
-    
+
+section "Size of Values (for induction)"
+  
+primrec vsize :: "val \<Rightarrow> nat" and esize :: "entry \<Rightarrow> nat" and fsize :: "func \<Rightarrow> nat" where
+"vsize (VNat n) = 1" |
+"vsize (VFun t) = 1 + fsize t" |
+"esize (v\<mapsto>v') = 1+ vsize v + vsize v'" |
+"fsize [] = 0" |
+"fsize (e#t) = 1+ esize e + fsize t"
+
 end
