DenotSem/Determ.thy
@@ -2,6 +2,27 @@ theory Determ
   imports Denot ValuesProps
 begin
 
+theorem deterministic:
+  "\<lbrakk> v \<in> \<lbrakk>e\<rbrakk>\<rho>; v' \<in> \<lbrakk>e\<rbrakk>\<rho>; val_env \<rho>; val_env \<rho>' \<rbrakk> \<Longrightarrow> v \<squnion> v' \<in> \<lbrakk>e\<rbrakk>(\<rho> \<squnion> \<rho>')"
+proof (induction e arbitrary: v v' \<rho> \<rho>')
+  case (EVar x)
+  then show ?case 
+next
+  case (ENat x)
+  then show ?case sorry
+next
+  case (ELam e)
+  then show ?case sorry
+next
+  case (EApp e1 e2)
+  then show ?case sorry
+next
+  case (EPrim x1a e1 e2)
+  then show ?case sorry
+next
+  case (EIf e1 e2 e3)
+  then show ?case sorry
+qed  
 
 
 end
