DenotSem/ValuesProps.thy
@@ -1,23 +1,286 @@
 theory ValuesProps
   imports Values
 begin
+  
+section "Facts about Value Sizes"
+  
+lemma val_size_mem: fixes e::entry assumes e_t: "e \<in> set t" shows "esize e < fsize t"
+  using e_t apply (induction t arbitrary: e)
+   apply force
+  apply simp apply (erule disjE)
+   apply arith    
+  apply (subgoal_tac "esize e < fsize t") prefer 2 apply blast
+  apply arith
+  done
 
-lemma fun_le_subset: "set t1 \<subseteq> set t2 \<Longrightarrow> t1 \<sqsubseteq> t2"
+lemma val_size_mem_l: assumes v12_t: "v1\<mapsto>v2 \<in> set t" shows "vsize v1 < fsize t"
+  using v12_t val_size_mem[of "v1\<mapsto>v2" t] by auto
+    
+lemma val_size_mem_r: assumes v12_t: "v1\<mapsto>v2 \<in> set t" shows "vsize v2 < fsize t"
+  using v12_t val_size_mem[of "v1\<mapsto> v2" t] by auto
+    
+section "More stuff"    
+
+  (*
+thm val_le_entry_le_fun_le_fun_in.induct
+  
+lemma fun_in_induct:
+  assumes base: "(\<And>p t. p \<in> set t \<Longrightarrow> P p t)" and
+    IH: "(\<And>p1 t p2. p1 in t \<Longrightarrow> P p1 t \<Longrightarrow> p1 \<sqsubseteq> p2 \<Longrightarrow> P p2 t)" and
+    prem: "p in f" 
+  shows "P p f"    
+proof -
+  let ?P1 = "\<lambda>v v'. True" and ?P2 = "\<lambda>p p'. True" and ?P3 = "\<lambda>f f'. True" and
+    ?P4 = "\<lambda>p f. P p f"
+  show ?thesis
+    using val_le_entry_le_fun_le_fun_in.induct[of ?P1 ?P3 ?P2 ?P4] base IH prem by blast
+qed
+  
+lemma fun_in_inv: "p in f \<Longrightarrow> \<exists> p'. p' \<in> set f \<and> p' \<sqsubseteq> p"
+  apply (induction rule: fun_in_induct)
+  
+    
+    
+lemma fun_le_mem: "\<lbrakk> p \<in> set f; VFun f \<sqsubseteq> VFun f'\<rbrakk> \<Longrightarrow> \<exists> p'. p \<sqsubseteq> p'"
+  apply clarify
+  apply (induction f arbitrary: p f')
+   apply force
+   apply auto
+   
+    
+lemma fun_le_intro: "\<lbrakk> \<forall>p. p |\<in>| f \<longrightarrow> (\<exists>p'. p' |\<in>| f' \<and> p \<sqsubseteq> p') \<rbrakk> \<Longrightarrow> VFun f \<sqsubseteq> VFun f'"    
+  by auto 
+*)
+
+lemma fun_le_subset: fixes f::func shows "set f \<subseteq> set f' \<Longrightarrow> f \<sqsubseteq> f'"
+  by (induction f arbitrary: f') auto
+
+lemma le_refl_aux:
+    "(\<forall> v. n = vsize v \<longrightarrow> v \<sqsubseteq> v)
+   \<and> (\<forall> p. n = esize p \<longrightarrow> p \<sqsubseteq> p) 
+   \<and> (\<forall> f. n = fsize f \<longrightarrow> f \<sqsubseteq> f)"
+proof (induction n rule: nat_less_induct)
+  case (1 n)
+  show ?case apply (rule conjI) apply clarify defer apply (rule conjI) apply clarify defer
+     apply clarify defer
+  proof -
+    fix v assume n: "n = vsize v"
+    show "v \<sqsubseteq> v"
+    proof (cases v)
+    case (VNat k)
+      then show ?thesis by blast
+    next
+      case (VFun t)
+      have "fsize t < n" using n VFun by simp
+      then show ?thesis using 1 VFun by auto
+    qed
+  next
+    fix p assume n: "n = esize p"
+    obtain v v' where p: "p = v \<mapsto> v'" by (cases p) auto
+    have "vsize v < n" using n p by auto
+    then have 2: "v \<sqsubseteq> v" using 1 by blast
+    have "vsize v' < n" using n p by auto
+    then have 3: "v' \<sqsubseteq> v'" using 1 by blast        
+    show "p \<sqsubseteq> p" using 2 3 p by blast
+  next
+    fix f assume n: "n = fsize f"
+    show "f \<sqsubseteq> f"
+    proof (cases f)
+      case Nil
+      then show ?thesis by auto
+    next
+      case (Cons p f')
+      have "fsize f' < n" using n Cons by auto
+      then have 2: "f' \<sqsubseteq> f'" using 1 Cons by auto
+      show ?thesis using 2 Cons apply simp apply (rule ins_le) defer
+          apply (rule fun_le_subset) apply force apply auto done
+    qed
+  qed
+qed
+  
+proposition val_le_refl[simp]: fixes v::val shows "v \<sqsubseteq> v" 
+  using le_refl_aux by blast
+  
+lemma val_le_trans_aux: fixes v2::val 
+  assumes n_vs2: "n = vsize v2"
+  shows "\<lbrakk> v1 \<sqsubseteq> v2; v2 \<sqsubseteq> v3 \<rbrakk> \<Longrightarrow> v1 \<sqsubseteq> v3" using n_vs2
+proof (induction n arbitrary: v1 v2 v3 rule: nat_less_induct)
+  case (1 n v1 v2 v3)
+  show ?case
+  proof (cases v1)
+    case (VNat n1)
+    with 1 show ?thesis by auto 
+  next
+    case (VFun t1) from VFun have v1: "v1 = VFun t1" .
+    show ?thesis
+    proof (cases v2)
+      case (VNat n2)
+      with VFun 1 have "False" by auto thus ?thesis ..
+    next
+      case (VFun t2) from VFun have v2: "v2 = VFun t2" .
+      show ?thesis
+      proof (cases v3)
+        case (VNat n3) with v1 1 have "False" by auto thus ?thesis ..
+      next
+        case (VFun t3)
+        show ?thesis using VFun v1 v2
+        proof clarify
+          fix v11 v11' assume v11_t1: "(v11,v11') |\<in>| t1"
+          from v11_t1 1(2) v1 v2 obtain v22 v22' where v22_t2: "(v22,v22') |\<in>| t2" 
+            and v2_v1: "v22 \<sqsubseteq> v11" and v1p_v2p: "v11' \<sqsubseteq> v22'" by blast
+          from v22_t2 1(3) v2 VFun obtain v33 v33' where v33_t3: "(v33,v33') |\<in>| t3"
+            and v3_v2: "v33 \<sqsubseteq> v22" and v2p_v3p: "v22' \<sqsubseteq> v33'" by blast
+          have "vsize v22 < fsize t2" using v22_t2 val_size_mem_l by blast
+          from this have s22_n: "vsize v22 < n" using v2 1(4) by auto   
+          have v3_v1: "v33 \<sqsubseteq> v11" using 1(1)
+            apply (erule_tac x="vsize v22" in allE) apply (erule impE) using s22_n apply blast
+              using v3_v2 v2_v1 by blast
+          have "vsize v22' < fsize t2" using v22_t2 val_size_mem_r by blast
+          from this have s22p_n: "vsize v22' < n" using v2 1(4) by auto   
+          have v1_v3: "v11' \<sqsubseteq> v33'" using 1(1)
+            apply (erule_tac x="vsize v22'" in allE) apply (erule impE) using s22p_n apply blast
+            using v1p_v2p v2p_v3p by blast 
+          from v3_v1 v1_v3 v33_t3
+          show "\<exists>v33 v33'. (v33, v33') |\<in>| t3 \<and> v33 \<sqsubseteq> v11 \<and> v11' \<sqsubseteq> v33'" by blast
+        qed
+      qed
+    qed
+  qed
+qed
+
+proposition val_le_trans[trans]: fixes v2::val shows "\<lbrakk> v1 \<sqsubseteq> v2; v2 \<sqsubseteq> v3 \<rbrakk> \<Longrightarrow> v1 \<sqsubseteq> v3"
+  using val_le_trans_aux by blast
+    
+
+
+  
+lemma consis_and_not_consis:
+  "(v ~ v' \<longrightarrow> \<not> (v !~ v')) \<and> (v !~ v' \<longrightarrow> \<not>(v ~ v'))"
+  apply (induction rule: consistent_inconsistent.induct) apply force+ done
+
+lemma consis_or_not_aux: assumes vs: "n = vsize v" shows "v ~ v' \<or> v !~ v'"
+  using vs apply (induction n  arbitrary: v v' rule: nat_less_induct)
+  apply (case_tac v)
+   apply (case_tac v')
+    apply force
+   apply force
+  apply (case_tac v')
+   apply force
+proof -
+  fix n v v' x2 x2a
+  assume IH: "\<forall>m<n. \<forall>x. m = vsize x \<longrightarrow> (\<forall>xa. x ~ xa \<or> x !~ xa)"
+    and n: "n = vsize v"
+    and v: "v = VFun x2" and vp: "v' = VFun x2a"
+  show "v ~ v' \<or> v !~ v'"
+  proof (cases "v !~ v'")
+    case True
+    then show ?thesis by blast
+  next
+    case False hence nc: "\<not> (v !~ v')" .
+    from v vp have "v ~ v'" apply simp apply (rule vfun_consis) apply (rule allI)+
+        apply (rule impI) apply (erule conjE)
+    proof -
+      fix v1 v1' v2 v2' assume 1: "v1\<mapsto> v1' \<in> set x2" and 2: "v2\<mapsto> v2' \<in> set x2a"
+      have 3: "vsize v1 < vsize (VFun x2)" using 1 val_size_mem_l[of v1 v1' x2] by auto 
+      from IH 3 n v have "v1 ~ v2 \<or> v1 !~ v2" by blast
+      from this show "(v1 ~ v2 \<and> v1' ~ v2') \<or> v1 !~ v2"
+      proof
+        assume v1_v2: "v1 ~ v2"
+        have 4: "vsize v1' < vsize (VFun x2)" using 1 val_size_mem_r[of v1 v1' x2] by auto 
+        have "v1' ~ v2' \<or> v1' !~ v2'" using IH 4 n v by blast
+        from this show ?thesis 
+        proof
+          assume "v1' ~ v2'" from v1_v2 this show ?thesis by blast
+        next
+          assume "v1' !~ v2'" 
+          then have "v !~ v'" using v1_v2 1 2 v vp by blast 
+          with nc have "False" ..
+          from this show ?thesis ..
+        qed
+      next
+        assume "v1 !~ v2"
+        then show ?thesis by blast
+      qed
+    qed
+    then show ?thesis by blast
+  qed
+qed
+    
+lemma consis_not[intro]: "\<not>(v !~ v') \<Longrightarrow> v ~ v'"
+  using consis_or_not_aux by blast 
+    
+lemma not_consis[intro]: "v ~ v' \<Longrightarrow> \<not> (v !~ v')" 
+  using consis_and_not_consis by blast
+
+lemma consis_refl[intro!]: "is_val v \<Longrightarrow> v ~ v"
+  apply (induction rule: is_val.induct)
+   apply blast
+  apply (simp only: is_fun_def)
+  apply (rule vfun_consis)
+  apply (rule allI)+ apply (rule impI)+ apply (erule conjE)+
+  apply (case_tac "v1 ~ v2") apply force apply blast 
+  done
+
+lemma consis_symm_aux:
+  "(v ~ v' \<longrightarrow> v' ~ v) \<and> (v !~ v' \<longrightarrow> v' !~ v)"
+  by (induction rule: consistent_inconsistent.induct) force+
+
+lemma consis_symm[sym]: "v ~ v' \<Longrightarrow> v' ~ v" 
+  using consis_symm_aux by blast
+
+lemma inconsis_symm[sym]: "v !~ v' \<Longrightarrow> v' !~ v" 
+  using consis_symm_aux by blast
+   
+lemma env_refl[intro!]: fixes \<rho>::"val list" shows "\<rho> \<sqsubseteq> \<rho>"
+  unfolding env_le_def apply auto done
+  
+lemma env_le_ext[intro!]: fixes v::val and \<rho>::"val list" 
+  shows "\<lbrakk> v \<sqsubseteq> v'; \<rho> \<sqsubseteq> \<rho>' \<rbrakk> \<Longrightarrow> v#\<rho> \<sqsubseteq> v'#\<rho>'"
+  unfolding env_le_def apply auto apply (case_tac k) apply force apply force done
+
+lemma val_env_ext[intro!]: "\<lbrakk> is_val v; val_env \<rho> \<rbrakk> \<Longrightarrow> val_env (v#\<rho>)"
+  unfolding val_env_def apply auto apply (case_tac k) apply auto done
+ 
+lemma consis_refl[intro!]: "is_val v \<Longrightarrow> v ~ v"
+  apply (induction rule: is_val.induct)
+   apply blast
+  apply (simp only: is_fun_def)
+  apply (rule vfun_consis)
+  apply (rule allI)+ apply (rule impI)+ apply (erule conjE)+
+  apply (case_tac "v1 ~ v2") apply force apply blast 
+  done
+    
+lemma consis_env_refl[intro!]: "val_env \<rho> \<Longrightarrow> consis_env \<rho> \<rho>"
+  apply (induction \<rho>) apply force
+  apply (rule consis_env_cons)
+   unfolding val_env_def apply (erule_tac x=0 in allE) apply force
+  apply (subgoal_tac "\<forall>k<length \<rho>. is_val (\<rho> ! k)") apply force 
+    apply clarify apply (erule_tac x="Suc k" in allE) apply auto done
+    
+lemma consis_length: "\<lbrakk> consis_env \<rho> \<rho>' \<rbrakk> \<Longrightarrow> length \<rho> = length \<rho>'"
+  apply (induction rule: consis_env.induct)
+   apply auto done
+
+lemma lookup_consis[intro]: "\<lbrakk> consis_env \<rho> \<rho>'; x < length \<rho> \<rbrakk> \<Longrightarrow> \<rho>!x ~ \<rho>'!x"
+  apply (induction arbitrary: x rule: consis_env.induct )
+   apply force apply (case_tac x) apply auto done
+
+lemma fun_le_subset: fixes t1::"func" shows "set t1 \<subseteq> set t2 \<Longrightarrow> t1 \<sqsubseteq> t2"
  by (induction t1) auto  
   
-lemma fun_le_append1: "t1 \<sqsubseteq> t1 @ t2"
+lemma fun_le_append1: fixes t1::"func" shows "t1 \<sqsubseteq> t1 @ t2"
 proof -
   have "set t1 \<subseteq> set (t1 @ t2)" by auto
   then show ?thesis using fun_le_subset by blast
 qed
   
-lemma fun_le_append2: "t1 \<sqsubseteq> t2 @ t1"
+lemma fun_le_append2: fixes t1::"func" shows "t1 \<sqsubseteq> t2 @ t1"
 proof -
   have "set t1 \<subseteq> set (t2 @ t1)" by auto
   then show ?thesis using fun_le_subset by blast
 qed
 
-lemma fun_append_le: fixes t1::"entry list" and t1'::"entry list"
+lemma fun_append_le: fixes t1::"func" and t1'::"func"
   assumes t1_t2: "t1 \<sqsubseteq> t2" and t1p_t2: "t1' \<sqsubseteq> t2" shows "t1 @ t1' \<sqsubseteq> t2"    
   using t1_t2 t1p_t2 by (induction t1 arbitrary: t1' t2) auto
     
